# Saved by TopBraid on Mon Mar 29 16:21:46 BST 2010
# baseURI: http://ontology.earthster.org/eco/alloc
# imports: http://ontology.earthster.org/eco/core

@prefix :        <http://ontology.earthster.org/eco/alloc#> .
@prefix rdfs:    <http://www.w3.org/2000/01/rdf-schema#> .
@prefix owl:     <http://www.w3.org/2002/07/owl#> .
@prefix xsd:     <http://www.w3.org/2001/XMLSchema#> .
@prefix rdf:     <http://www.w3.org/1999/02/22-rdf-syntax-ns#> .
@prefix eco:     <http://ontology.earthster.org/eco/core#> .
@prefix alloc:   <http://ontology.earthster.org/eco/alloc#> .

<http://ontology.earthster.org/eco/alloc>
      a       owl:Ontology ;
      rdfs:comment """The Earthsterâ„¢ ECO Allocation Ontology

This ontology is an extension to the ECO ontology.  It defines a number of allocation method.

To the extent possible under law, New Earth  has waived all copyright and related or neighboring rights to http://ontology.earthster.org/eco/alloc. This work is published from United States. """^^xsd:string ;
      owl:imports <http://ontology.earthster.org/eco/core> ;
      owl:versionInfo "In early development: subject to incompatible change without notice."^^xsd:string .

:AllocationMethodEconomicCausility
      a       owl:Class ;
      rdfs:comment """A class of allocations determined by economic causality.

This class is currently a placeholder.  Its definition should define exactly what it means by economic causality."""^^xsd:string ;
      rdfs:subClassOf eco:Allocation .

:AllocationMethodPhysicalCausality
      a       owl:Class ;
      rdfs:comment """A class of allocations determined by a method of physical causality.

This is currently a placeholder class until the method is specified more precisely."""^^xsd:string ;
      rdfs:subClassOf eco:Allocation .

:AllocationMethodUndefined
      a       owl:Class ;
      rdfs:comment "A class of allocations whose method is undefined."^^xsd:string ;
      rdfs:subClassOf eco:Allocation .
