# Saved by TopBraid on Mon Mar 29 16:22:45 BST 2010
# baseURI: http://ontology.earthster.org/eco/attribute
# imports: http://ontology.earthster.org/eco/core

@prefix :        <http://ontology.earthster.org/eco/attribute#> .
@prefix rdfs:    <http://www.w3.org/2000/01/rdf-schema#> .
@prefix owl:     <http://www.w3.org/2002/07/owl#> .
@prefix xsd:     <http://www.w3.org/2001/XMLSchema#> .
@prefix rdf:     <http://www.w3.org/1999/02/22-rdf-syntax-ns#> .
@prefix attr:    <http://ontology.earthster.org/eco/attribute#> .
@prefix eco:     <http://ontology.earthster.org/eco/core#> .

<http://ontology.earthster.org/eco/attribute>
      a       owl:Ontology ;
      rdfs:comment """The Earthsterâ„¢ ECO attribute ontology.

This is an extention ontology for ECO that defines the RATIO attribute definition class.

To the extent possible under law, New Earth  has waived all copyright and related or neighboring rights to http://ontology.earthster.org/eco/attribute. This work is published from United States. """^^xsd:string ;
      owl:imports <http://ontology.earthster.org/eco/core> ;
      owl:versionInfo "In early development: subject to incompatible change without notice."^^xsd:string .

:RatioAttributeDefinition
      a       owl:Class ;
      rdfs:comment """A class of attribute definitions that are a ratio of two quantified effects.

Examples of ratio attribute definitions include the ratio of child to all labour used in producing a product."""^^xsd:string ;
      rdfs:label "Ratio attribute"^^xsd:string ;
      rdfs:subClassOf eco:AttributeDefinition ;
      rdfs:subClassOf
              [ a       owl:Restriction ;
                owl:maxCardinality "1"^^xsd:int ;
                owl:onProperty :hasDivisorUnit
              ] ;
      rdfs:subClassOf
              [ a       owl:Restriction ;
                owl:cardinality "1"^^xsd:int ;
                owl:onProperty :hasDivisor
              ] ;
      rdfs:subClassOf
              [ a       owl:Restriction ;
                owl:cardinality "1"^^xsd:int ;
                owl:onProperty :hasDividend
              ] ;
      rdfs:subClassOf
              [ a       owl:Restriction ;
                owl:maxCardinality "1"^^xsd:int ;
                owl:onProperty :hasDividendUnit
              ] .

:hasDividend
      a       owl:ObjectProperty ;
      rdfs:comment "hasDividend relates a ratio attribute definition to the effect whose value is the dividend of the ratio."^^xsd:string ;
      rdfs:domain :RatioAttributeDefinition ;
      rdfs:label "has dividend"^^xsd:string ;
      rdfs:range eco:EffectAggregationCategory .

:hasDividendUnit
      a       owl:ObjectProperty ;
      rdfs:comment "hasDividendUnit relates a ratio attribute definition to the units in which its dividend are measured."^^xsd:string ;
      rdfs:domain :RatioAttributeDefinition ;
      rdfs:label "has dividend unit"^^xsd:string ;
      rdfs:range eco:UnitOfMeasure .

:hasDivisor
      a       owl:ObjectProperty ;
      rdfs:comment "hasDivisor relates a Ratio attribute definition to the effect aggregation category that is the divisor of the ratio."^^xsd:string ;
      rdfs:domain :RatioAttributeDefinition ;
      rdfs:label "has divisor"^^xsd:string ;
      rdfs:range eco:EffectAggregationCategory .

:hasDivisorUnit
      a       owl:ObjectProperty ;
      rdfs:comment "hasDivisorUnit relates a ratio attribute definition to the units in which the divisor should be measured."^^xsd:string ;
      rdfs:domain :RatioAttributeDefinition ;
      rdfs:label "has divisor unit"^^xsd:string ;
      rdfs:range eco:UnitOfMeasure .
