# Saved by TopBraid on Fri May 14 12:43:54 BST 2010
# baseURI: http://ontology.earthster.org/eco/ecoinvent
# imports: http://ontology.earthster.org/eco/core
# imports: http://ontology.earthster.org/eco/impact
# imports: http://www.w3.org/2004/02/skos/core

@prefix :        <http://ontology.earthster.org/eco/ecoinvent#> .
@prefix core:    <http://ontology.earthster.org/eco/core#> .
@prefix ei:      <http://ontology.earthster.org/eco/ecoinvent#> .
@prefix impact:  <http://ontology.earthster.org/eco/impact#> .
@prefix owl:     <http://www.w3.org/2002/07/owl#> .
@prefix rdf:     <http://www.w3.org/1999/02/22-rdf-syntax-ns#> .
@prefix rdfs:    <http://www.w3.org/2000/01/rdf-schema#> .
@prefix skos:    <http://www.w3.org/2004/02/skos/core#> .
@prefix xsd:     <http://www.w3.org/2001/XMLSchema#> .

<http://ontology.earthster.org/eco/ecoinvent>
      rdf:type owl:Ontology ;
      rdfs:comment """The Earthsterâ„¢ ECO extension ontology for EcoInvent.

This is an eco extension ontology that describes concepts in the EcoInvent database.

To the extent possible under law, New Earth  has waived all copyright and related or neighboring rights to http://ontology.earthster.org/eco/ecoinvent. This work is published from United States."""^^xsd:string ;
      owl:imports <http://ontology.earthster.org/eco/impact> , <http://www.w3.org/2004/02/skos/core> , <http://ontology.earthster.org/eco/core> ;
      owl:versionInfo "In early development: subject to change without notice."^^xsd:string .

ei:ID
      rdf:type owl:DatatypeProperty ;
      rdfs:comment "indicates the ei identifier for an entity"^^xsd:string ;
      rdfs:label "flow ID"^^xsd:string .

ei:LandOrSeaCategory
      rdf:type owl:Class ;
      rdfs:comment """A category of land or sea.

Examples of categories of land or sea include arable land and forestry.

No identity criteria are defined for categories of land or sea."""^^xsd:string ;
      rdfs:label "Land category"^^xsd:string ;
      rdfs:subClassOf owl:Thing .

ei:Occupation
      rdf:type owl:Class ;
      rdfs:comment """An occupation of land.

Examples of occupation include occupation of arable land.

A necessary condition for two occupations to be identical is that they have the same occupationCategories."""^^xsd:string ;
      rdfs:label "Occupation"^^xsd:string ;
      rdfs:subClassOf core:Effect .

ei:Transformation
      rdf:type owl:Class ;
      rdfs:comment """A transformation is an effect that transforms land.

Examples of transformations transform land from slag to arable.

A necessary condition for two transformations to be identical is that they have the same transformation from and two land categories."""^^xsd:string ;
      rdfs:label "Transformation"^^xsd:string ;
      rdfs:subClassOf core:Effect .

ei:VolumeOccupation
      rdf:type owl:Class ;
      rdfs:comment """A kind of effect.

Examples of volume occupation include volumes occupied with radioactive waste.

A necessary condition for two volume oxccupations to be identical is that they are occupied with the same category of thing."""^^xsd:string ;
      rdfs:label "Volume occupied"^^xsd:string ;
      rdfs:subClassOf core:Effect .

ei:VolumeOccupationCategory
      rdf:type owl:Class ;
      rdfs:comment """A category for the effect VolumeOccupation.

Examples of volume occupation category include occupied with radioactive waste.

No identity criteria are defined for volume occupation categories."""^^xsd:string ;
      rdfs:label "Volume occupation category"^^xsd:string ;
      rdfs:subClassOf owl:Thing .

ei:arable
      rdf:type ei:LandOrSeaCategory ;
      rdfs:comment ""^^xsd:string ;
      rdfs:label "arable"^^xsd:string ;
      skos:broader ei:land .

ei:arableNonIrrigated
      rdf:type ei:LandOrSeaCategory ;
      rdfs:comment ""^^xsd:string ;
      rdfs:label "arable non irrigated"^^xsd:string ;
      skos:broader ei:arable .

ei:arableNonIrrigatedDiverseIntensive
      rdf:type ei:LandOrSeaCategory ;
      rdfs:comment ""^^xsd:string ;
      rdfs:label "arable non irrigated diverse intensive"^^xsd:string ;
      skos:broader ei:arable .

ei:arableNonIrrigatedFallow
      rdf:type ei:LandOrSeaCategory ;
      rdfs:comment ""^^xsd:string ;
      rdfs:label "arable non irrigated fallow"^^xsd:string ;
      skos:broader ei:arable .

ei:arableNonIrrigatedMonotoneIntensive
      rdf:type ei:LandOrSeaCategory ;
      rdfs:comment ""^^xsd:string ;
      rdfs:label "arable non irrigated monotone intensive"^^xsd:string ;
      skos:broader ei:arable .

ei:category1Label
      rdf:type owl:DatatypeProperty ;
      rdfs:label "category1Label"^^xsd:string ;
      ei:category1Label "indicate the category 1 label for a resource."^^xsd:string .

ei:category2Label
      rdf:type owl:DatatypeProperty ;
      rdfs:comment "Indicates the category 2 label used by EcoInvent."^^xsd:string ;
      rdfs:label "category 2 label"^^xsd:string .

ei:constructionSite
      rdf:type ei:LandOrSeaCategory ;
      rdfs:comment ""^^xsd:string ;
      rdfs:label "construction site"^^xsd:string ;
      skos:broader ei:land .

ei:dumpSite
      rdf:type ei:LandOrSeaCategory ;
      rdfs:comment ""^^xsd:string ;
      rdfs:label "dump site"^^xsd:string ;
      skos:broader ei:land .

ei:dumpSiteBenthos
      rdf:type ei:LandOrSeaCategory ;
      rdfs:comment ""^^xsd:string ;
      rdfs:label "dump site benthos"^^xsd:string ;
      skos:broader ei:dumpSite .

ei:dumpSiteInertMaterialLandfill
      rdf:type ei:LandOrSeaCategory ;
      rdfs:comment ""^^xsd:string ;
      rdfs:label "dump site inert material landfill"^^xsd:string ;
      skos:broader ei:dumpSite .

ei:dumpSiteResidualMaterialLandfill
      rdf:type ei:LandOrSeaCategory ;
      rdfs:label "dump site residual material landfill"^^xsd:string ;
      skos:broader ei:dumpSite .

ei:dumpSiteSanitaryLandfill
      rdf:type ei:LandOrSeaCategory ;
      rdfs:label "dump site sanitary landfill"^^xsd:string ;
      skos:broader ei:dumpSite .

ei:dumpSiteSlagCompartment
      rdf:type ei:LandOrSeaCategory ;
      rdfs:label "dump site slag compartment"^^xsd:string ;
      skos:broader ei:dumpSite .

ei:finalRepositoryLowLevelRadioactiveWaste
      rdf:type ei:VolumeOccupationCategory ;
      rdfs:label "final repository for low activity radioactive waste"^^xsd:string .

ei:finalRepositoryRadioactiveWaste
      rdf:type ei:VolumeOccupationCategory ;
      rdfs:label "final repository radioactive waste"^^xsd:string .

ei:forest
      rdf:type ei:LandOrSeaCategory ;
      rdfs:comment ""^^xsd:string ;
      rdfs:label "forest"^^xsd:string ;
      skos:broader ei:land .

ei:forestExtensive
      rdf:type ei:LandOrSeaCategory ;
      rdfs:comment ""^^xsd:string ;
      rdfs:label "forest extensive"^^xsd:string ;
      skos:broader ei:forest .

ei:forestIntensive
      rdf:type ei:LandOrSeaCategory ;
      rdfs:comment ""^^xsd:string ;
      rdfs:label "forest intensive"^^xsd:string ;
      skos:broader ei:land .

ei:forestIntensiveNormal
      rdf:type ei:LandOrSeaCategory ;
      rdfs:comment ""^^xsd:string ;
      rdfs:label "forest intensive normal"^^xsd:string ;
      skos:broader ei:forestIntensive .

ei:forestIntensiveShortCycle
      rdf:type ei:LandOrSeaCategory ;
      rdfs:comment ""^^xsd:string ;
      rdfs:label "forest intensive short cutting"^^xsd:string ;
      skos:broader ei:forestIntensive .

ei:forestIntensiveclearCutting
      rdf:type ei:LandOrSeaCategory ;
      rdfs:comment ""^^xsd:string ;
      rdfs:label "forest intensiveclear cutting"^^xsd:string ;
      skos:broader ei:forestIntensive .

ei:hasOccupationCategory
      rdf:type owl:ObjectProperty ;
      rdfs:comment "relates an occupation to a category of land that is occupied."^^xsd:string ;
      rdfs:label "has land category"^^xsd:string ;
      skos:broader ei:land .

ei:hasTransformationFromCategory
      rdf:type owl:ObjectProperty ;
      rdfs:comment "relates a transformation effect to the category of land that is transformed from."^^xsd:string ;
      rdfs:domain ei:Transformation ;
      rdfs:label "has transformation from category"^^xsd:string ;
      rdfs:range ei:LandOrSeaCategory .

ei:hasTransformationToCategory
      rdf:type owl:ObjectProperty ;
      rdfs:comment "relates a transformation effect to the land category that is transformed to."^^xsd:string ;
      rdfs:domain ei:Transformation ;
      rdfs:label "has transformation to category"^^xsd:string ;
      rdfs:range ei:LandOrSeaCategory .

ei:hasVolumeOccupationCategory
      rdf:type owl:ObjectProperty ;
      rdfs:comment "relates a volume occupation effect to the category of occupation."^^xsd:string ;
      rdfs:domain ei:VolumeOccupation ;
      rdfs:label "has volume occupation category"^^xsd:string ;
      rdfs:range ei:VolumeOccupationCategory .

ei:heterogeneousArgicultural
      rdf:type ei:LandOrSeaCategory ;
      rdfs:comment ""^^xsd:string ;
      rdfs:label "heterogeneous argicultural"^^xsd:string ;
      skos:broader ei:land .

ei:industrial
      rdf:type ei:LandOrSeaCategory ;
      rdfs:comment ""^^xsd:string ;
      rdfs:label "industrial"^^xsd:string ;
      skos:broader ei:land .

ei:industrialBenthos
      rdf:type ei:LandOrSeaCategory ;
      rdfs:comment ""^^xsd:string ;
      rdfs:label "industrial benthos"^^xsd:string ;
      skos:broader ei:land .

ei:industrialBuiltup
      rdf:type ei:LandOrSeaCategory ;
      rdfs:comment ""^^xsd:string ;
      rdfs:label "industrial builtup"^^xsd:string ;
      skos:broader ei:industrial .

ei:industrialVegetation
      rdf:type ei:LandOrSeaCategory ;
      rdfs:comment ""^^xsd:string ;
      rdfs:label "industrial vegetation"^^xsd:string ;
      skos:broader ei:industrial .

ei:label
      rdf:type owl:DatatypeProperty ;
      rdfs:comment "indicates the label used by EcoInvent to represent an entity."^^xsd:string ;
      rdfs:label "ei label"^^xsd:string .

ei:land
      rdf:type ei:LandOrSeaCategory ;
      rdfs:comment ""^^xsd:string ;
      rdfs:label "land"^^xsd:string ;
      skos:broader ei:landOrSea .

ei:landOrSea
      rdf:type ei:LandOrSeaCategory ;
      rdfs:comment ""^^xsd:string ;
      rdfs:label "Land or sea"^^xsd:string .

ei:mineralExtraction
      rdf:type ei:LandOrSeaCategory ;
      rdfs:comment ""^^xsd:string ;
      rdfs:label "mineral extraction"^^xsd:string ;
      skos:broader ei:land .

ei:nameLabel
      rdf:type owl:DatatypeProperty ;
      rdfs:comment "Indicates the name given to an item in EcoInvent."^^xsd:string ;
      rdfs:label "name label"^^xsd:string .

ei:pastureAndMeadow
      rdf:type ei:LandOrSeaCategory ;
      rdfs:comment ""^^xsd:string ;
      rdfs:label "pasture and meadow"^^xsd:string ;
      skos:broader ei:land .

ei:pastureAndMeadowExtensive
      rdf:type ei:LandOrSeaCategory ;
      rdfs:comment ""^^xsd:string ;
      rdfs:label "pasture and meadow extensive"^^xsd:string ;
      skos:broader ei:pastureAndMeadow .

ei:pastureAndMeadowIntensive
      rdf:type ei:LandOrSeaCategory ;
      rdfs:comment ""^^xsd:string ;
      rdfs:label "pasture and meadow intensive"^^xsd:string ;
      skos:broader ei:pastureAndMeadow .

ei:permanentCrop
      rdf:type ei:LandOrSeaCategory ;
      rdfs:comment ""^^xsd:string ;
      rdfs:label "permanent crop"^^xsd:string ;
      skos:broader ei:land .

ei:permanentCropFruit
      rdf:type ei:LandOrSeaCategory ;
      rdfs:comment ""^^xsd:string ;
      rdfs:label "permanent crop fruit"^^xsd:string ;
      skos:broader ei:permanentCrop .

ei:permanentCropFruitExtensive
      rdf:type ei:LandOrSeaCategory ;
      rdfs:comment ""^^xsd:string ;
      rdfs:label "permanent crop fruit extensive"^^xsd:string ;
      skos:broader ei:permanentCropFruit .

ei:permanentCropFruitIntensive
      rdf:type ei:LandOrSeaCategory ;
      rdfs:comment ""^^xsd:string ;
      rdfs:label "permanent crop fruit intensive"^^xsd:string ;
      skos:broader ei:permanentCropFruit .

ei:permanentCropVine
      rdf:type ei:LandOrSeaCategory ;
      rdfs:comment ""^^xsd:string ;
      rdfs:label "permanent crop vine"^^xsd:string ;
      skos:broader ei:permanentCrop .

ei:permanentCropVineExtensive
      rdf:type ei:LandOrSeaCategory ;
      rdfs:comment ""^^xsd:string ;
      rdfs:label "permanent crop vine extensive"^^xsd:string ;
      skos:broader ei:permanentCropVine .

ei:permanentCropVineIntensive
      rdf:type ei:LandOrSeaCategory ;
      rdfs:comment ""^^xsd:string ;
      rdfs:label "permanent crop vine intensive"^^xsd:string ;
      skos:broader ei:permanentCropVine .

ei:resevoir
      rdf:type ei:VolumeOccupationCategory ;
      rdfs:label "resevoir"^^xsd:string .

ei:seaOrOcean
      rdf:type ei:LandOrSeaCategory ;
      rdfs:comment ""^^xsd:string ;
      rdfs:label "sea or ocean"^^xsd:string ;
      skos:broader ei:landOrSea .

ei:shrubLandSclerophyllous
      rdf:type ei:LandOrSeaCategory ;
      rdfs:comment ""^^xsd:string ;
      rdfs:label "shrub land sclerophyllous"^^xsd:string ;
      skos:broader ei:land .

ei:trafficAreaRailEmbankment
      rdf:type ei:LandOrSeaCategory ;
      rdfs:comment ""^^xsd:string ;
      rdfs:label "traffic area rail embankment"^^xsd:string ;
      skos:broader ei:land .

ei:trafficAreaRailNetwork
      rdf:type ei:LandOrSeaCategory ;
      rdfs:comment ""^^xsd:string ;
      rdfs:label "traffic area rail network"^^xsd:string ;
      skos:broader ei:land .

ei:trafficAreaRoadEmbankment
      rdf:type ei:LandOrSeaCategory ;
      rdfs:comment ""^^xsd:string ;
      rdfs:label "traffic area road embankment"^^xsd:string ;
      skos:broader ei:land .

ei:trafficAreaRoadNetwork
      rdf:type ei:LandOrSeaCategory ;
      rdfs:comment ""^^xsd:string ;
      rdfs:label "traffic area road network"^^xsd:string ;
      skos:broader ei:land .

ei:tropicalRainForest
      rdf:type ei:LandOrSeaCategory ;
      rdfs:comment ""^^xsd:string ;
      rdfs:label "tropical rain forest"^^xsd:string ;
      skos:broader ei:land .

ei:undergroundDeposit
      rdf:type ei:VolumeOccupationCategory ;
      rdfs:label "underground deposit"^^xsd:string .

ei:urbanContinuouslyBuilt
      rdf:type ei:LandOrSeaCategory ;
      rdfs:comment ""^^xsd:string ;
      rdfs:label "urban continuously built"^^xsd:string ;
      skos:broader ei:land .

ei:urbanDiscontinuouslyBuilt
      rdf:type ei:LandOrSeaCategory ;
      rdfs:comment ""^^xsd:string ;
      rdfs:label "urban discontinuously built"^^xsd:string ;
      skos:broader ei:land .

ei:waterBodyArtificial
      rdf:type ei:LandOrSeaCategory ;
      rdfs:comment ""^^xsd:string ;
      rdfs:label "water body artificial"^^xsd:string ;
      skos:broader ei:land .

ei:waterCourseArtificial
      rdf:type ei:LandOrSeaCategory ;
      rdfs:comment ""^^xsd:string ;
      rdfs:label "water course artificial"^^xsd:string ;
      skos:broader ei:land .

impact:CD-CML2001-AbioticDepletion
      ei:nameLabel "depletion of abiotic resources"^^xsd:string .

impact:CD-CML2001-Acidification
      ei:nameLabel "average European"^^xsd:string .

impact:CD-CML2001-Acidification-alt1
      ei:nameLabel "generic"^^xsd:string .

impact:CD-CML2001-ClimateChange
      ei:nameLabel "GWP 100a"^^xsd:string .

impact:CD-CML2001-ClimateChange-alt1
      ei:nameLabel "GWP 20a"^^xsd:string .

impact:CD-CML2001-ClimateChange-alt2
      ei:nameLabel "GWP 500a"^^xsd:string .

impact:CD-CML2001-ClimateChange-alt3
      ei:nameLabel "upper limit of net GWP"^^xsd:string .

impact:CD-CML2001-ClimateChange-alt4
      ei:nameLabel "lower limit of net GWP"^^xsd:string .

impact:CD-CML2001-Eutrophication
      ei:nameLabel "generic"^^xsd:string .

impact:CD-CML2001-Eutrophication-alt1
      ei:nameLabel "average European"^^xsd:string .

impact:CD-CML2001-FreshwaterAquaticEcotoxicity
      ei:nameLabel "FAETP infinite"^^xsd:string .

impact:CD-CML2001-FreshwaterAquaticEcotoxicity-alt1
      ei:nameLabel "FAETP 100a"^^xsd:string .

impact:CD-CML2001-FreshwaterAquaticEcotoxicity-alt2
      ei:nameLabel "FAETP 20a"^^xsd:string .

impact:CD-CML2001-FreshwaterAquaticEcotoxicity-alt3
      ei:nameLabel "FAETP 500a"^^xsd:string .

impact:CD-CML2001-HumanToxicity
      ei:nameLabel "HTP infinite"^^xsd:string .

impact:CD-CML2001-HumanToxicity-alt1
      ei:nameLabel "HTP 20a"^^xsd:string .

impact:CD-CML2001-HumanToxicity-alt2
      ei:nameLabel "HTP 100a"^^xsd:string .

impact:CD-CML2001-HumanToxicity-alt3
      ei:nameLabel "HTP 500a"^^xsd:string .

impact:CD-CML2001-MarineAquaticEcotoxicity
      ei:nameLabel "MAETP infinite"^^xsd:string .

impact:CD-CML2001-MarineAquaticEcotoxicity-alt1
      ei:nameLabel "MAETP 100a"^^xsd:string .

impact:CD-CML2001-MarineAquaticEcotoxicity-alt2
      ei:nameLabel "MAETP 20a"^^xsd:string .

impact:CD-CML2001-MarineAquaticEcotoxicity-alt3
      ei:nameLabel "MAETP 500a"^^xsd:string .

impact:CD-CML2001-OzoneLayerDepletion
      ei:nameLabel "ODP steady state"^^xsd:string .

impact:CD-CML2001-OzoneLayerDepletion-alt1
      ei:nameLabel "ODP 5a"^^xsd:string .

impact:CD-CML2001-OzoneLayerDepletion-alt2
      ei:nameLabel "ODP 10a"^^xsd:string .

impact:CD-CML2001-OzoneLayerDepletion-alt3
      ei:nameLabel "ODP 15a"^^xsd:string .

impact:CD-CML2001-OzoneLayerDepletion-alt4
      ei:nameLabel "ODP 20a"^^xsd:string .

impact:CD-CML2001-OzoneLayerDepletion-alt5
      ei:nameLabel "ODP 25a"^^xsd:string .

impact:CD-CML2001-OzoneLayerDepletion-alt6
      ei:nameLabel "ODP 30a"^^xsd:string .

impact:CD-CML2001-OzoneLayerDepletion-alt7
      ei:nameLabel "ODP 40a"^^xsd:string .

impact:CD-CML2001-PhotoOxidantFomation
      ei:nameLabel "high NOx POCP"^^xsd:string .

impact:CD-CML2001-PhotoOxidantFomation-alt1
      ei:nameLabel "MIR"^^xsd:string .

impact:CD-CML2001-PhotoOxidantFomation-alt2
      ei:nameLabel "MOIR"^^xsd:string .

impact:CD-CML2001-PhotoOxidantFomation-alt3
      ei:nameLabel "EBIR"^^xsd:string .

impact:CD-CML2001-PhotoOxidantFomation-alt4
      ei:nameLabel "low NOx POCP"^^xsd:string .

impact:CD-CML2001-TerrestrialEcotoxicity
      ei:nameLabel "TAETP infinite"^^xsd:string .

impact:CD-CML2001-TerrestrialEcotoxicity-alt1
      ei:nameLabel "TAETP 100a"^^xsd:string .

impact:CD-CML2001-TerrestrialEcotoxicity-alt2
      ei:nameLabel "TAETP 20a"^^xsd:string .

impact:CD-CML2001-TerrestrialEcotoxicity-alt3
      ei:nameLabel "TAETP 500a"^^xsd:string .

impact:CML2001
      ei:category1Label "CML 2001"^^xsd:string .

impact:abioticDepletion
      ei:category2Label "resources"^^xsd:string .

impact:ozoneLayerDepletion
      ei:category2Label "stratospheric ozone depletion"^^xsd:string .

impact:photoOxidantFormation
      ei:category2Label "photochemical oxidation (summer smog)"^^xsd:string .
