# Saved by TopBraid on Wed Jun 09 08:55:34 BST 2010
# baseURI: http://ontology.earthster.org/eco/fasc
# imports: http://ontology.earthster.org/eco/core
# imports: http://www.w3.org/2004/02/skos/core
# imports: http://ontology.earthster.org/eco/ecoinvent

@prefix :        <http://ontology.earthster.org/eco/fasc#> .
@prefix eco:     <http://ontology.earthster.org/eco/core#> .
@prefix ecoinvent:  <http://ontology.earthster.org/eco/ecoinvent#> .
@prefix owl:     <http://www.w3.org/2002/07/owl#> .
@prefix rdf:     <http://www.w3.org/1999/02/22-rdf-syntax-ns#> .
@prefix rdfs:    <http://www.w3.org/2000/01/rdf-schema#> .
@prefix skos:    <http://www.w3.org/2004/02/skos/core#> .
@prefix xsd:     <http://www.w3.org/2001/XMLSchema#> .

<http://ontology.earthster.org/eco/fasc>
      rdf:type owl:Ontology ;
      rdfs:comment """The Earthsterâ„¢ ECO Effect Aggregation Categories ontology.

This is an eco extension ontology that defines the class FlowAggregationCategory to represent the concept of a flow as a pair of substance and compartment.

It is an extension point for defining other kinds of common aggregation categories.

To the extent possible under law, New Earth  has waived all copyright and related or neighboring rights to http://ontology.earthster.org/eco/fasc. This work is published from United States. """^^xsd:string ;
      owl:imports <http://www.w3.org/2004/02/skos/core> , <http://ontology.earthster.org/eco/ecoinvent> , <http://ontology.earthster.org/eco/core> ;
      owl:versionInfo "In early development: subject to incompatible change without notice."^^xsd:string .

:BioticSubstanceSource
      rdf:type owl:Class ;
      rdfs:comment ""^^xsd:string ;
      rdfs:label "Biotic substance source"^^xsd:string ;
      rdfs:subClassOf :SubstanceSource ;
      owl:disjointWith :FossilSubstanceSource .

:Compartment
      rdf:type owl:Class ;
      rdfs:comment """A compartment is a classification of locations in the ecosphere.  Compartments are used to indicate the kind of source or destination of elementary flows.

Examples of compartments include urban air and ground water.

A necessary condition for compartments to be identical is that they have identical values for their medium and population density properties, if such values exist."""^^xsd:string ;
      rdfs:label "Compartment"^^xsd:string ;
      rdfs:seeAlso :FlowAggregationCategory ;
      rdfs:subClassOf owl:Thing ;
      rdfs:subClassOf
              [ rdf:type owl:Restriction ;
                owl:minCardinality "0"^^xsd:nonNegativeInteger ;
                owl:onProperty :hasLongevity
              ] ;
      rdfs:subClassOf
              [ rdf:type owl:Restriction ;
                owl:minCardinality "0"^^xsd:int ;
                owl:onProperty :hasCompartmentPopulationDensity
              ] ;
      rdfs:subClassOf
              [ rdf:type owl:Restriction ;
                owl:minCardinality "0"^^xsd:int ;
                owl:onProperty :hasCompartmentMedium
              ] .

:CompartmentMedium
      rdf:type owl:Class ;
      rdfs:comment """A compartment medium is kind of classification of a compartment.

Examples of compartment media include Air and Water.

No identity criteria are defined for compartment media."""^^xsd:string ;
      rdfs:label "Compartment medium"^^xsd:string ;
      rdfs:subClassOf owl:Thing .

:CompartmentPopulationDensity
      rdf:type owl:Class ;
      rdfs:comment """A compartment population density is used to categorise compartments.

Examples of compartment population density include Urban and Rural.

No identity criteria are defined for compartment population densities."""^^xsd:string ;
      rdfs:label "Compartment population density"^^xsd:string ;
      rdfs:subClassOf owl:Thing .

:FlowAggregationCategory
      rdf:type owl:Class ;
      rdfs:comment """A flow aggregation category is pair consisting of a flowable and a compartment.

Examples of flow aggregation categories include carbon dioxide to urban air.

A necessary and sufficient condition for two flow aggregation categories to be identical is that they have the same flowable and the same compartment."""^^xsd:string ;
      rdfs:label "Flow aggregation category"^^xsd:string ;
      rdfs:subClassOf eco:EffectAggregationCategory ;
      owl:equivalentClass
              [ rdf:type owl:Class ;
                owl:intersectionOf ([ rdf:type owl:Restriction ;
                            owl:cardinality "1"^^xsd:int ;
                            owl:onProperty :hasFlowable
                          ] [ rdf:type owl:Restriction ;
                            owl:cardinality "1"^^xsd:int ;
                            owl:onProperty :hasCompartment
                          ])
              ] .

:FossilSubstanceSource
      rdf:type owl:Class ;
      rdfs:comment ""^^xsd:string ;
      rdfs:label "Fossil substance source"^^xsd:string ;
      rdfs:subClassOf :SubstanceSource ;
      owl:disjointWith :BioticSubstanceSource .

:LongTerm
      rdf:type owl:Class ;
      rdfs:comment ""^^xsd:string ;
      rdfs:label "Long term"^^xsd:string ;
      rdfs:subClassOf :Longevity ;
      owl:equivalentClass
              [ rdf:type owl:Class ;
                owl:oneOf (:longTerm)
              ] .

:Longevity
      rdf:type owl:Class ;
      rdfs:comment """Longevity is a value class indicating the longevity of an emission.

Example of longevity include long term and not long term.

No identity criteria are defined for longevity."""^^xsd:string ;
      rdfs:label "Longevity"^^xsd:string ;
      rdfs:subClassOf owl:Thing ;
      owl:equivalentClass
              [ rdf:type owl:Class ;
                owl:unionOf (:LongTerm :NotLongTerm)
              ] .

:NotLongTerm
      rdf:type owl:Class ;
      rdfs:comment "A class of values of longevity."^^xsd:string ;
      rdfs:label "Not long term"^^xsd:string ;
      rdfs:subClassOf :Longevity ;
      owl:disjointWith :LongTerm .

:SubstanceSource
      rdf:type owl:Class ;
      rdfs:comment """A  substance source is classification of the source of a substance.

Examples of substance sources are fossil and biotic.

No identity criteria are defined for substance sources."""^^xsd:string ;
      rdfs:label "Substance source"^^xsd:string ;
      rdfs:subClassOf owl:Thing .

:agriculturalSoil
      rdf:type :CompartmentMedium ;
      rdfs:comment ""^^xsd:string ;
      rdfs:label "agricultural soil"^^xsd:string ;
      skos:broader :soil .

:air  rdf:type :CompartmentMedium ;
      rdfs:comment ""^^xsd:string ;
      rdfs:label "air"^^xsd:string .

:biotic
      rdf:type :BioticSubstanceSource ;
      rdfs:comment ""^^xsd:string ;
      rdfs:label "biotic"^^xsd:string .

:forestrySoil
      rdf:type :CompartmentMedium ;
      rdfs:comment ""^^xsd:string ;
      rdfs:label "forestry soil"^^xsd:string ;
      skos:broader :nonAgriculturalSoil .

:fossil
      rdf:type :FossilSubstanceSource ;
      rdfs:comment ""^^xsd:string ;
      rdfs:label "fossil"^^xsd:string .

:fossilWater
      rdf:type :CompartmentMedium ;
      rdfs:comment ""^^xsd:string ;
      rdfs:label "fossil water"^^xsd:string ;
      skos:broader :water .

:freshWater
      rdf:type :CompartmentMedium ;
      rdfs:comment ""^^xsd:string ;
      rdfs:label "fresh water"^^xsd:string ;
      skos:broader :water .

:groundWater
      rdf:type :CompartmentMedium ;
      rdfs:comment ""^^xsd:string ;
      rdfs:label "ground water"^^xsd:string ;
      skos:broader :freshWater .

:hasCompartment
      rdf:type owl:ObjectProperty ;
      rdfs:comment "hasCompartment indicates a compartment related to a resource.  It may be used to relate a flow aggregation category to a compartment."^^xsd:string ;
      rdfs:label "to compartment"^^xsd:string ;
      rdfs:range :Compartment .

:hasCompartmentMedium
      rdf:type owl:ObjectProperty ;
      rdfs:comment "hasCompartmentMedium relates a compartment to its medium."^^xsd:string ;
      rdfs:domain :Compartment ;
      rdfs:label "has compartment medium"^^xsd:string ;
      rdfs:range :CompartmentMedium .

:hasCompartmentPopulationDensity
      rdf:type owl:ObjectProperty ;
      rdfs:comment "hasCompartmentPopulationDensity relates a compartment to its population density."^^xsd:string ;
      rdfs:domain :Compartment ;
      rdfs:label "has compartment population density"^^xsd:string ;
      rdfs:range :CompartmentPopulationDensity .

:hasEffect
      rdf:type owl:ObjectProperty ;
      rdfs:comment "relates an effect aggregation category to the effect it aggregates."^^xsd:string ;
      rdfs:domain eco:EffectAggregationCategory ;
      rdfs:label "has effect"^^xsd:string ;
      rdfs:range eco:Effect .

:hasFlowable
      rdf:type owl:ObjectProperty ;
      rdfs:comment "hasFlowable relates a flow aggregation category to a flowable."^^xsd:string ;
      rdfs:domain :FlowAggregationCategory ;
      rdfs:label "has flowable"^^xsd:string ;
      rdfs:range eco:Flowable .

:hasLongevity
      rdf:type owl:ObjectProperty ;
      rdfs:comment "hasLongevity indicates the longevity of a compartment"^^xsd:string ;
      rdfs:domain :Compartment ;
      rdfs:label "has longevity"^^xsd:string ;
      rdfs:range :Longevity .

:hasOccupationCategory
      rdf:type owl:ObjectProperty ;
      rdfs:comment "relates an EffectAggregationCategory to a land category category"^^xsd:string ;
      rdfs:domain eco:EffectAggregationCategory ;
      rdfs:label "has occupation category"^^xsd:string ;
      rdfs:range ecoinvent:LandOrSeaCategory .

:hasSubstanceSource
      rdf:type owl:ObjectProperty , owl:FunctionalProperty ;
      rdfs:comment "hasSubstanceSource indicates the source of a substance."^^xsd:string ;
      rdfs:domain eco:Substance ;
      rdfs:label "has substance source"^^xsd:string ;
      rdfs:range :SubstanceSource .

:hasTransformationFromCategory
      rdf:type owl:ObjectProperty ;
      rdfs:comment "relates an effect aggregation category to the land transformation category the transfromation is from."^^xsd:string ;
      rdfs:domain eco:EffectAggregationCategory ;
      rdfs:label "has transformation from category"^^xsd:string ;
      rdfs:range ecoinvent:LandOrSeaCategory .

:hasTransformationToCategory
      rdf:type owl:ObjectProperty ;
      rdfs:comment "relates an effect aggregation category to the land transformation category the transfromation is to."^^xsd:string ;
      rdfs:domain eco:EffectAggregationCategory ;
      rdfs:label "has transformation to category"^^xsd:string ;
      rdfs:range ecoinvent:LandOrSeaCategory .

:hasVolumeOccupationCategory
      rdf:type owl:ObjectProperty ;
      rdfs:comment "relates a volume occupation effect to a category of volume occupation."^^xsd:string ;
      rdfs:label "has volume occupation category"^^xsd:string .

:highAir
      rdf:type :CompartmentMedium ;
      rdfs:comment ""^^xsd:string ;
      rdfs:label "high air"^^xsd:string ;
      skos:broader :air .

:highPopulationDensity
      rdf:type :CompartmentPopulationDensity ;
      rdfs:comment ""^^xsd:string ;
      rdfs:label "high population density"^^xsd:string .

:industrySoil
      rdf:type :CompartmentMedium ;
      rdfs:comment ""^^xsd:string ;
      rdfs:label "industry soil"^^xsd:string ;
      skos:broader :nonAgriculturalSoil .

:lakeWater
      rdf:type :CompartmentMedium ;
      rdfs:comment "lake water is fresh water"^^xsd:string ;
      rdfs:label "lake water"^^xsd:string ;
      skos:broader :freshWater .

:longTerm
      rdf:type :LongTerm ;
      rdfs:comment ""^^xsd:string ;
      rdfs:label "long term"^^xsd:string .

:lowAir
      rdf:type :CompartmentMedium ;
      rdfs:comment ""^^xsd:string ;
      rdfs:label "low air"^^xsd:string ;
      skos:broader :air .

:lowPopulationDensity
      rdf:type :CompartmentPopulationDensity ;
      rdfs:comment ""^^xsd:string ;
      rdfs:label "low population density"^^xsd:string .

:nonAgriculturalSoil
      rdf:type :CompartmentMedium ;
      rdfs:comment ""^^xsd:string ;
      rdfs:label "non agricultural soil"^^xsd:string ;
      skos:broader :soil .

:notLongTerm
      rdf:type :NotLongTerm ;
      rdfs:comment ""^^xsd:string ;
      rdfs:label "not long term"^^xsd:string .

:resource
      rdf:type :CompartmentMedium ;
      rdfs:comment ""^^xsd:string ;
      rdfs:label "Resource"^^xsd:string .

:resourceBiotic
      rdf:type :CompartmentMedium ;
      rdfs:comment ""^^xsd:string ;
      rdfs:label "resource biotic"^^xsd:string ;
      skos:broader :resource .

:resourceInAir
      rdf:type :CompartmentMedium ;
      rdfs:comment ""^^xsd:string ;
      rdfs:label "resource in air"^^xsd:string ;
      skos:broader :resource .

:resourceInGround
      rdf:type :CompartmentMedium ;
      rdfs:comment ""^^xsd:string ;
      rdfs:label "resource in ground"^^xsd:string ;
      skos:broader :resource .

:resourceInWater
      rdf:type :CompartmentMedium ;
      rdfs:comment ""^^xsd:string ;
      rdfs:label "resource water"^^xsd:string ;
      skos:broader :resource .

:resourceLand
      rdf:type :CompartmentMedium ;
      rdfs:comment ""^^xsd:string ;
      rdfs:label "resource land"^^xsd:string ;
      skos:broader :resource .

:riverWater
      rdf:type :CompartmentMedium ;
      rdfs:comment ""^^xsd:string ;
      rdfs:label "river water"^^xsd:string ;
      skos:broader :freshWater .

:seaWater
      rdf:type :CompartmentMedium ;
      rdfs:comment ""^^xsd:string ;
      rdfs:label "sea water"^^xsd:string ;
      skos:broader :water .

:soil
      rdf:type :CompartmentMedium ;
      rdfs:comment ""^^xsd:string ;
      rdfs:label "soil"^^xsd:string .

:surfaceWater
      rdf:type :CompartmentMedium ;
      rdfs:comment ""^^xsd:string ;
      rdfs:label "surface water"^^xsd:string ;
      skos:broader :freshWater .

:tropoStratoSphere
      rdf:type :CompartmentMedium ;
      rdfs:comment "higher toposphere or lower stratosphere"^^xsd:string ;
      rdfs:label "tropo strato sphere"^^xsd:string ;
      skos:broader :air .

:water
      rdf:type :CompartmentMedium ;
      rdfs:comment ""^^xsd:string ;
      rdfs:label "water"^^xsd:string .
