# Saved by TopBraid on Sun Apr 04 12:27:38 BST 2010
# baseURI: http://ontology.earthster.org/eco/ilcd
# imports: http://ontology.earthster.org/eco/core

@prefix ilcd:    <http://ontology.earthster.org/eco/ilcd#> .
@prefix rdfs:    <http://www.w3.org/2000/01/rdf-schema#> .
@prefix owl:     <http://www.w3.org/2002/07/owl#> .
@prefix xsd:     <http://www.w3.org/2001/XMLSchema#> .
@prefix rdf:     <http://www.w3.org/1999/02/22-rdf-syntax-ns#> .
@prefix core:    <http://ontology.earthster.org/eco/core#> .

<http://ontology.earthster.org/eco/ilcd>
      a       owl:Ontology ;
      rdfs:comment """An Earthsterâ„¢ ECO extension ontology for ILCD.

An ontology of concepts specific to ILCD.

To the extent possible under law, New Earth  has waived all copyright and related or neighboring rights to http://ontology.earthster.org/eco/ilcd. This work is published from United States."""^^xsd:string ;
      owl:imports <http://ontology.earthster.org/eco/core> ;
      owl:versionInfo "In early development: subject to incompatible change without notice"^^xsd:string .

ilcd:EME
      a       owl:Class ;
      rdfs:comment "A value partition of flowables into elements, materials or energy."^^xsd:string ;
      rdfs:label "EME"^^xsd:string ;
      rdfs:subClassOf owl:Thing .

ilcd:EMEelement
      a       owl:Class ;
      rdfs:comment ""^^xsd:string ;
      rdfs:label "EMEelement"^^xsd:string ;
      rdfs:subClassOf ilcd:EME ;
      owl:disjointWith ilcd:EMEenergy , ilcd:EMEmaterial ;
      owl:equivalentClass
              [ a       owl:Class ;
                owl:oneOf (ilcd:emeElement)
              ] .

ilcd:EMEenergy
      a       owl:Class ;
      rdfs:comment ""^^xsd:string ;
      rdfs:label "EMEenergy"^^xsd:string ;
      rdfs:subClassOf ilcd:EME ;
      owl:disjointWith ilcd:EMEelement , ilcd:EMEmaterial ;
      owl:equivalentClass
              [ a       owl:Class ;
                owl:oneOf (ilcd:emeEnergy)
              ] .

ilcd:EMEmaterial
      a       owl:Class ;
      rdfs:comment ""^^xsd:string ;
      rdfs:label "EMEmaterial"^^xsd:string ;
      rdfs:subClassOf ilcd:EME ;
      owl:disjointWith ilcd:EMEenergy , ilcd:EMEelement ;
      owl:equivalentClass
              [ a       owl:Class ;
                owl:oneOf (ilcd:emeMaterial)
              ] .

ilcd:emeElement
      a       ilcd:EME ;
      rdfs:comment ""^^xsd:string ;
      rdfs:label "eme element"^^xsd:string .

ilcd:emeEnergy
      a       ilcd:EME ;
      rdfs:comment ""^^xsd:string ;
      rdfs:label "eme energy"^^xsd:string .

ilcd:emeMaterial
      a       ilcd:EME ;
      rdfs:comment ""^^xsd:string ;
      rdfs:label "eme material"^^xsd:string .

ilcd:hasILCDUUID
      a       owl:DatatypeProperty ;
      rdfs:comment "hasILCDUUID indicates a UUID allocated by ILCD."^^xsd:string ;
      rdfs:label "has ILCDUUID"^^xsd:string ;
      rdfs:subPropertyOf core:hasUUID .

ilcd:ilcdLabel
      a       owl:DatatypeProperty ;
      rdfs:comment "links a resource to an ILCD specific label for that resource."^^xsd:string ;
      rdfs:label "ilcd label"^^xsd:string .
